trillium/program_logic/traces.v
@@ -109,6 +109,91 @@ Section system_trace.
 
 End system_trace.
 
+Definition inf_execution_trace Λ := inflist (olocale Λ * cfg Λ).
+
+Section inf_execution_trace.
+  Context {Λ : language}.
+
+  Definition inf_exec_prepend ζ (c : cfg Λ)
+             (iex : inf_execution_trace Λ) : inf_execution_trace Λ :=
+    ((ζ, c) :: iex)%inflist.
+
+  CoInductive valid_inf_exec :
+    execution_trace Λ → inf_execution_trace Λ → Prop :=
+  | valid_inf_exec_singleton ex :
+      valid_exec ex → valid_inf_exec ex []%inflist
+  | valid_inf_exec_step ex c c' iex ζ:
+      valid_exec ex →
+      trace_ends_in ex c →
+      locale_step c ζ c' →
+      valid_inf_exec (trace_extend ex ζ c') iex →
+      valid_inf_exec ex (inf_exec_prepend ζ c' iex).
+
+End inf_execution_trace.
+
+Definition inf_auxiliary_trace (M : Model) := inflist ((mlabel $ M) * M).
+
+Definition inf_auxtr_prepend {M : Model} ℓ (δ : M) (atr : inf_auxiliary_trace M) :=
+  infcons (ℓ,δ) atr.
+
+CoInductive valid_inf_system_trace {Λ M}
+            (Ψ : execution_trace Λ → auxiliary_trace M → Prop) :
+  execution_trace Λ → auxiliary_trace M →
+  inf_execution_trace Λ → inf_auxiliary_trace M → Prop :=
+| valid_inf_system_trace_singleton ex atr :
+    Ψ ex atr →
+    valid_inf_system_trace Ψ ex atr []%inflist []%inflist
+| valid_inf_system_trace_step ex atr c c' δ' iex iatr ζ ℓ:
+    Ψ ex atr →
+    trace_ends_in ex c →
+    locale_step c ζ c' →
+    valid_inf_system_trace
+      Ψ (trace_extend ex ζ c') (trace_extend atr ℓ δ') iex iatr →
+    valid_inf_system_trace
+      Ψ ex atr (inf_exec_prepend ζ c' iex) (inf_auxtr_prepend ℓ δ' iatr).
+
+Lemma valid_inf_system_trace_inv {Λ M}
+      (Ψ : execution_trace Λ → auxiliary_trace M → Prop) ex atr iex itr :
+  valid_inf_system_trace Ψ ex atr iex itr →
+  Ψ ex atr.
+Proof. by inversion 1. Qed.
+
+  Lemma valid_inf_exec_adjust {Λ : language} {ex: execution_trace Λ} {c iex ζ} :
+    valid_inf_exec ex ((ζ, c) :: iex)%inflist →
+    valid_inf_exec (trace_extend ex ζ c) iex.
+  Proof. inversion 1; done. Qed.
+
+  Lemma valid_inf_exe_valid_exec {Λ : language} {ex: execution_trace Λ} iex :
+    valid_inf_exec ex iex → valid_exec ex.
+  Proof. by destruct 1. Qed.
+  Lemma valid_inf_exe_take_drop {Λ : language} {ex: execution_trace Λ} iex n :
+    valid_inf_exec ex iex → valid_inf_exec (ex +trl+ inflist_take n iex) (inflist_drop n iex).
+  Proof.
+    revert ex iex; induction n as [|n IHn]; intros ex iex Hvl; simpl; first done.
+    destruct iex as [|[??]]; simpl; first done.
+    apply IHn.
+    apply valid_inf_exec_adjust; done.
+  Qed.
+
+  Lemma valid_system_trace_start_or_contract {Λ : language} {M: Model}
+    (ex: execution_trace Λ) (atr: auxiliary_trace M) :
+    valid_system_trace ex atr →
+    (ex = {tr[trace_first ex]} ∧ atr = {tr[trace_first atr]}) ∨
+    (∃ ex' atr' oζ ℓ, trace_contract ex oζ ex' ∧ trace_contract atr ℓ atr').
+  Proof. rewrite /trace_contract; inversion 1; simplify_eq; eauto 10. Qed.
+
+  Lemma valid_inf_exec_prepend_valid_exec_extend {Λ : language}
+    (ex: execution_trace Λ) c iex ζ:
+    valid_inf_exec ex (inf_exec_prepend ζ c iex) →
+    valid_exec (trace_extend ex ζ c).
+  Proof.
+    inversion 1 as [|???????? Hex]; simplify_eq.
+    inversion Hex; done.
+  Qed.
+
+  Definition trace_extend_uncurry {M: Model}
+    (tr: auxiliary_trace M) xy := trace_extend tr xy.2 xy.1.
+
 Section simulation.
   Context {Λ : language} {M : Model}.
   Variable (labels_match : olocale Λ → mlabel M → Prop).
@@ -218,56 +303,7 @@ Section simulation.
 
 End simulation.
 
-Definition inf_execution_trace Λ := inflist (olocale Λ * cfg Λ).
-
-Section inf_execution_trace.
-  Context {Λ : language}.
-
-  Definition inf_exec_prepend ζ (c : cfg Λ)
-             (iex : inf_execution_trace Λ) : inf_execution_trace Λ :=
-    ((ζ, c) :: iex)%inflist.
-
-  CoInductive valid_inf_exec :
-    execution_trace Λ → inf_execution_trace Λ → Prop :=
-  | valid_inf_exec_singleton ex :
-      valid_exec ex → valid_inf_exec ex []%inflist
-  | valid_inf_exec_step ex c c' iex ζ:
-      valid_exec ex →
-      trace_ends_in ex c →
-      locale_step c ζ c' →
-      valid_inf_exec (trace_extend ex ζ c') iex →
-      valid_inf_exec ex (inf_exec_prepend ζ c' iex).
-
-End inf_execution_trace.
-
-Definition inf_auxiliary_trace (M : Model) := inflist ((mlabel $ M) * M).
-
-Definition inf_auxtr_prepend {M : Model} ℓ (δ : M) (atr : inf_auxiliary_trace M) :=
-  infcons (ℓ,δ) atr.
-
-CoInductive valid_inf_system_trace {Λ M}
-            (Ψ : execution_trace Λ → auxiliary_trace M → Prop) :
-  execution_trace Λ → auxiliary_trace M →
-  inf_execution_trace Λ → inf_auxiliary_trace M → Prop :=
-| valid_inf_system_trace_singleton ex atr :
-    Ψ ex atr →
-    valid_inf_system_trace Ψ ex atr []%inflist []%inflist
-| valid_inf_system_trace_step ex atr c c' δ' iex iatr ζ ℓ:
-    Ψ ex atr →
-    trace_ends_in ex c →
-    locale_step c ζ c' →
-    valid_inf_system_trace
-      Ψ (trace_extend ex ζ c') (trace_extend atr ℓ δ') iex iatr →
-    valid_inf_system_trace
-      Ψ ex atr (inf_exec_prepend ζ c' iex) (inf_auxtr_prepend ℓ δ' iatr).
-
-Lemma valid_inf_system_trace_inv {Λ M}
-      (Ψ : execution_trace Λ → auxiliary_trace M → Prop) ex atr iex itr :
-  valid_inf_system_trace Ψ ex atr iex itr →
-  Ψ ex atr.
-Proof. by inversion 1. Qed.
-
-Section simulation.
+Section simulation2.
   Context {Λ : language} {M : Model}
           (φ : execution_trace Λ → auxiliary_trace M → Prop).
 
@@ -276,20 +312,6 @@ Section simulation.
   Implicit Types atr : auxiliary_trace M.
   Implicit Types ζ : olocale Λ.
   Implicit Types ℓ : mlabel M.
-
-  Lemma valid_system_trace_start_or_contract ex atr :
-    valid_system_trace ex atr →
-    (ex = {tr[trace_first ex]} ∧ atr = {tr[trace_first atr]}) ∨
-    (∃ ex' atr' oζ ℓ, trace_contract ex oζ ex' ∧ trace_contract atr ℓ atr').
-  Proof. rewrite /trace_contract; inversion 1; simplify_eq; eauto 10. Qed.
-
-  Lemma valid_inf_exec_prepend_valid_exec_extend ex c iex ζ:
-    valid_inf_exec ex (inf_exec_prepend ζ c iex) →
-    valid_exec (trace_extend ex ζ c).
-  Proof.
-    inversion 1 as [|???????? Hex]; simplify_eq.
-    inversion Hex; done.
-  Qed.
 
   Lemma produce_inf_aux_trace_next_aux_state_exists
         (ex : execution_trace Λ) (atr : auxiliary_trace M)
@@ -315,8 +337,6 @@ Section simulation.
     epsilon
       (produce_inf_aux_trace_next_aux_state_exists ex atr Hcsm c ζ iex Hvex).
 
-  Definition trace_extend_uncurry (tr: auxiliary_trace M) xy := trace_extend tr xy.2 xy.1.
-
   Lemma produce_inf_aux_trace_next_aux_state_continued_simulation
         (ex : execution_trace Λ) (atr : auxiliary_trace M)
         (Hcsm : continued_simulation φ ex atr)
@@ -332,23 +352,6 @@ Section simulation.
   Proof.
     rewrite /produce_inf_aux_trace_next_aux_state.
     apply epsilon_correct.
-  Qed.
-
-  Local Lemma valid_inf_exec_adjust {ex c iex ζ} :
-    valid_inf_exec ex ((ζ, c) :: iex)%inflist →
-    valid_inf_exec (trace_extend ex ζ c) iex.
-  Proof. inversion 1; done. Qed.
-
-  Lemma valid_inf_exe_valid_exec ex iex :
-    valid_inf_exec ex iex → valid_exec ex.
-  Proof. by destruct 1. Qed.
-  Lemma valid_inf_exe_take_drop ex iex n :
-    valid_inf_exec ex iex → valid_inf_exec (ex +trl+ inflist_take n iex) (inflist_drop n iex).
-  Proof.
-    revert ex iex; induction n as [|n IHn]; intros ex iex Hvl; simpl; first done.
-    destruct iex as [|[??]]; simpl; first done.
-    apply IHn.
-    apply valid_inf_exec_adjust; done.
   Qed.
 
   CoFixpoint produce_inf_aux_trace
@@ -403,4 +406,259 @@ Section simulation.
       econstructor; eauto using valid_system_trace_step.
   Qed.
 
-End simulation.
+End simulation2.
+
+Section simulation_cond.
+  Context {Λ : language} {M : Model}.
+  Variable (labels_match : olocale Λ → mlabel M → Prop).
+
+  Implicit Types ex : execution_trace Λ.
+  Implicit Types atr : auxiliary_trace M.
+
+  Definition continued_simulation_cond_pre
+             (φ : execution_trace Λ → auxiliary_trace M → Prop)
+             (C: execution_trace Λ → Prop)
+             (continued_simulation :
+                execution_trace Λ → auxiliary_trace M → Prop) :
+    execution_trace Λ → auxiliary_trace M → Prop :=
+    λ ex atr,
+      C ex ->
+      φ ex atr ∧
+      ∀ c c' ζ,
+        trace_ends_in ex c →
+        locale_step c ζ c' →
+        ∃ δ' ℓ, continued_simulation (trace_extend ex ζ c') (trace_extend atr ℓ δ').
+
+  Local Definition continued_simulation_cond_pre_curried
+        (φ : execution_trace Λ → auxiliary_trace M → Prop)
+        (C: execution_trace Λ → Prop) :
+    (execution_trace Λ * auxiliary_trace M → Prop) →
+    (execution_trace Λ * auxiliary_trace M → Prop) :=
+    λ ψ (exatr : execution_trace Λ * auxiliary_trace M),
+    (continued_simulation_cond_pre φ C (λ ex atr, ψ (ex, atr)) exatr.1 exatr.2).
+
+  Lemma continued_simulation_cond_pre_curried_mono
+        (φ : execution_trace Λ → auxiliary_trace M → Prop)
+        (C: execution_trace Λ → Prop) :
+    monotone (continued_simulation_cond_pre_curried φ C).
+  Proof.
+    intros P Q HPQ [ex atr].
+    intros ?.
+    intros PASS. specialize (H PASS) as [? HP].
+    split; [done|].
+    intros ?????.
+    edestruct HP as (?&?&?); eauto.
+  Qed.
+
+  Definition continued_simulation_cond
+    (φ : execution_trace Λ → auxiliary_trace M → Prop)
+    (C: execution_trace Λ → Prop) :=
+    λ ex atr, GFX (continued_simulation_cond_pre_curried φ C) (ex, atr).
+
+  Lemma continued_simulation_cond_unfold
+        (φ : execution_trace Λ → auxiliary_trace M → Prop)
+        (C: execution_trace Λ → Prop) ex atr :
+    continued_simulation_cond φ C ex atr ↔
+    continued_simulation_cond_pre φ C (continued_simulation_cond φ C) ex atr.
+  Proof.
+    symmetry; rewrite /continued_simulation_cond /=.
+    apply (λ H, GFX_fixpoint (continued_simulation_cond_pre_curried φ C) H (_, _)).
+    apply continued_simulation_cond_pre_curried_mono.
+  Qed.
+
+  Lemma continued_simulation_cond_rel Φ C ex tr
+    `{forall ex, Decision (C ex)}:
+    continued_simulation_cond Φ C ex tr → Φ ex tr ∨ ¬ C ex.
+  Proof.
+    rewrite continued_simulation_cond_unfold /continued_simulation_cond_pre.
+    destruct (decide (C ex)); [| tauto]. 
+    intuition.
+  Qed.
+
+  Definition filter_pref_closed (C: execution_trace Λ → Prop) :=
+    forall ex τ c, C (trace_extend ex τ c) -> C ex. 
+
+  Lemma continued_simulation_cond_next_aux_state_exists
+             (φ : execution_trace Λ → auxiliary_trace M → Prop)
+             C
+             (PCL: filter_pref_closed C)
+             `{forall ex, Decision (C ex)}
+             `{Inhabited (mlabel M)}
+             (ex : execution_trace Λ) (atr : auxiliary_trace M)
+             (c : cfg Λ) ζ:
+    continued_simulation_cond φ C ex atr →
+    valid_exec (trace_extend ex ζ c) →
+    ∃ δℓ, continued_simulation_cond φ C (trace_extend ex ζ c) (trace_extend atr δℓ.2 δℓ.1).
+  Proof using.
+    clear labels_match. 
+    rewrite continued_simulation_cond_unfold /continued_simulation_cond_pre.
+    destruct (decide (C (ex :tr[ ζ ]: c))) as [PASS' | FAIL'].
+    2: { intros _ _.
+         inversion H0 as [ℓ].
+         exists (trace_last atr, ℓ).
+         rewrite continued_simulation_cond_unfold /continued_simulation_cond_pre.
+         tauto. }
+    apply PCL in PASS'.
+    intros X Hvex. specialize (X PASS'). destruct X as (HΦ & Hext).
+    apply valid_exec_exec_extend_inv in Hvex as [Hvex (c1 & Hc1 & Hstep)].
+    edestruct Hext as (?&?&?); [done..|].
+    by eexists (_,_).
+  Qed.
+
+  Lemma simulation_cond_does_continue es σ δ φ C
+             (PCL: filter_pref_closed C)
+             `{forall ex, Decision (C ex)}
+             `{Inhabited (mlabel M)}:
+    continued_simulation_cond φ C (trace_singleton (es, σ)) (trace_singleton δ) →
+    ∀ ex, trace_starts_in ex (es, σ) →
+          valid_exec ex →
+          ∃ atr, trace_starts_in atr δ ∧ continued_simulation_cond φ C ex atr.
+  Proof.
+    intros Hsm ex Hexstr Hex.
+    induction Hex as [|? ? ? ? ? ? ? IHex].
+    - apply trace_singleton_starts_in_inv in Hexstr as ->.
+      exists (trace_singleton δ). done.
+    - destruct IHex as [atr [Hstarts Hsim]].
+      { eapply trace_extend_starts_in_inv; eauto. }
+      edestruct (continued_simulation_cond_next_aux_state_exists φ C PCL ex atr) as ([??]&?);
+        [done| |].
+      { econstructor; eauto. }
+      eexists. split; [|done].
+      by apply trace_extend_starts_in.
+  Qed.
+
+  (* TODO: its original version is unused? *)
+  (* Lemma continued_simulation_cond_impl (Φ Ψ: execution_trace Λ → auxiliary_trace M → Prop) C ex tr: *)
+  (*   (∀ ex tr, Φ ex tr → Ψ ex tr) → *)
+  (*   continued_simulation_cond Φ C ex tr → continued_simulation_cond Ψ C ex tr. *)
+  (* Proof. *)
+  (*   intros Himpl Hphi. *)
+  (*   rewrite /continued_simulation_cond /GFX. *)
+  (*   exists (λ '(ex, atr), continued_simulation_cond Φ C ex atr). *)
+  (*   split; [done|]. *)
+  (*   intros [? ?] ?. *)
+  (*   rewrite /continued_simulation_cond_pre_curried /continued_simulation_cond_pre /=. *)
+  (*   split. *)
+  (*   { eapply Himpl. *)
+  (*   rewrite /continued_simulation_cond /GFX in H.  *)
+
+  (*   unfold continued_simulation_cond_pre_curried, continued_simulation_cond_pre in H.  *)
+  (*     specialize (H H0).  *)
+  (*     eapply continued_simulation_cond_rel. } *)
+  (*   intros c c' ζ ? ?. *)
+  (*   move: H. *)
+  (*   rewrite continued_simulation_unfold /continued_simulation_pre. *)
+  (*   intros [? ?]. eauto. *)
+  (* Qed. *)
+
+End simulation_cond.
+
+Section simulation2.
+  Context {Λ : language} {M : Model}
+          (φ : execution_trace Λ → auxiliary_trace M → Prop)
+          (C: execution_trace Λ → Prop).
+
+  Context (PCL: filter_pref_closed C)
+    {C_DEC: forall ex, Decision (C ex)}
+    {ML_INH: Inhabited (mlabel M)}. 
+
+  Implicit Types ex : execution_trace Λ.
+  Implicit Types iex : inf_execution_trace Λ.
+  Implicit Types atr : auxiliary_trace M.
+  Implicit Types ζ : olocale Λ.
+  Implicit Types ℓ : mlabel M.
+
+  Lemma produce_inf_aux_trace_next_aux_state_cond_exists
+        (ex : execution_trace Λ) (atr : auxiliary_trace M)
+        (Hcsm : continued_simulation_cond φ C ex atr)
+        (c : cfg Λ)
+        (ζ: olocale Λ)
+        (iex : inf_execution_trace Λ)
+        (Hvex : valid_inf_exec ex (inf_exec_prepend ζ c iex)) :
+    ∃ δℓ, continued_simulation_cond φ C (trace_extend ex ζ c) (trace_extend atr δℓ.2 δℓ.1).
+  Proof.
+    eapply continued_simulation_cond_next_aux_state_exists; eauto. 
+    eapply valid_inf_exec_prepend_valid_exec_extend; eauto.
+  Qed.
+
+  Definition produce_inf_aux_trace_next_aux_state_cond
+             (ex : execution_trace Λ) (atr : auxiliary_trace M)
+             (Hcsm : continued_simulation_cond φ C ex atr)
+             (c : cfg Λ)
+             (ζ: olocale Λ)
+             (iex : inf_execution_trace Λ)
+             (Hvex : valid_inf_exec ex (inf_exec_prepend ζ c iex))
+    : (M * mlabel M)%type :=
+    epsilon
+      (produce_inf_aux_trace_next_aux_state_cond_exists ex atr Hcsm c ζ iex Hvex).
+
+  Lemma produce_inf_aux_trace_next_aux_state_continued_simulation_cond
+        (ex : execution_trace Λ) (atr : auxiliary_trace M)
+        (Hcsm : continued_simulation_cond φ C ex atr)
+        (c : cfg Λ)
+        (ζ: olocale Λ)
+        (iex : inf_execution_trace Λ)
+        (Hvex : valid_inf_exec ex (inf_exec_prepend ζ c iex)) :
+    continued_simulation_cond
+      φ C
+      (trace_extend ex ζ c)
+      (trace_extend_uncurry
+         atr (produce_inf_aux_trace_next_aux_state_cond ex atr Hcsm c ζ iex Hvex)).
+  Proof.
+    rewrite /produce_inf_aux_trace_next_aux_state_cond.
+    apply epsilon_correct.
+  Qed.
+
+  CoFixpoint produce_inf_aux_trace_cond
+          (ex : execution_trace Λ) (atr : auxiliary_trace M)
+          (Hcsm : continued_simulation_cond φ C ex atr)
+          (iex : inf_execution_trace Λ)
+          (Hvex : valid_inf_exec ex iex) :
+    inf_auxiliary_trace M :=
+    match iex as l return valid_inf_exec ex l → inf_auxiliary_trace M with
+    | [] => λ _, []
+    | (ζ, c) :: iex' =>
+      λ Hvex',
+      let δℓ :=
+          produce_inf_aux_trace_next_aux_state_cond ex atr Hcsm c ζ iex' Hvex'
+      in
+      (δℓ.2, δℓ.1) :: (produce_inf_aux_trace_cond
+              (trace_extend ex ζ c)
+              (trace_extend atr δℓ.2 δℓ.1)
+              (produce_inf_aux_trace_next_aux_state_continued_simulation_cond
+                 ex atr Hcsm c ζ iex' Hvex')
+              iex'
+              (valid_inf_exec_adjust Hvex'))
+    end%inflist Hvex.
+
+  Theorem produced_inf_aux_trace_valid_inf_cond
+          (ex : execution_trace Λ) (atr : auxiliary_trace M)
+          (Hst : valid_system_trace ex atr)
+          (Hcsm : continued_simulation_cond φ C ex atr)
+          (iex : inf_execution_trace Λ)
+          (Hvex : valid_inf_exec ex iex)
+    : valid_inf_system_trace
+        (continued_simulation_cond φ C)
+        ex atr
+        iex
+        (produce_inf_aux_trace_cond ex atr Hcsm iex Hvex).
+  Proof.
+    revert ex atr Hcsm Hst iex Hvex; cofix CIH; intros ex atr Hcsm Hst iex Hvex.
+    destruct iex as [|[ζ c] iex].
+    - rewrite [produce_inf_aux_trace_cond _ _ _ _ _]inflist_unfold_fold /=.
+      constructor; trivial.
+    - rewrite [produce_inf_aux_trace_cond _ _ _ _ _]inflist_unfold_fold /=.
+      pose proof (produce_inf_aux_trace_next_aux_state_continued_simulation_cond
+                    ex atr Hcsm c ζ iex Hvex) as Hcsm'.
+      assert (valid_system_trace
+                (ex :tr[ζ]: c)
+                (trace_extend_uncurry
+                   atr (produce_inf_aux_trace_next_aux_state_cond ex atr Hcsm c ζ iex Hvex)))
+             as Hst'.
+      { inversion Hvex; simplify_eq.
+        econstructor; try done. }
+      apply valid_system_trace_extend_inv in Hst' as (?&?&?&?).
+      econstructor; eauto using valid_system_trace_step.
+  Qed.
+
+End simulation2.
